\section{Question 1}
\subsection{a}
Illustrate the use of the Gauss reduction in obtaining the general solution of the following set of equations:

\begin{align}
	2x_1 + x_3 &= 4 \label{eq:I1} \\
	x_1 - 2x_2 + 2x_3 &= 7 \label{eq:I2} \\
	3x_1 + 2x_2 &= 1 \label{eq:I3}
\end{align}

We can solve this system using Gaussian elimination to obtain the general solution:

\begin{align*}
	2x_1 + 0x_2 + x_3 &= 4 \tag{1'} \\
	0x_1 + x_2 - \frac{1}{2}x_3 &= -\frac{5}{2} \tag{2'} \\
	0x_1 + 0x_2 + 0x_3 &= 0 \tag{3'}
\end{align*}

Now, we can express the solutions as follows:

\begin{align*}
	x_3 &= t \quad \text{(a free parameter)} \\
	x_2 &= -\frac{5}{2} + \frac{1}{2}t \\
	x_1 &= 2 - \frac{1}{2}t
\end{align*}

So, the general solution to the system of equations \eqref{eq:I1}, \eqref{eq:I2}, and \eqref{eq:I3} is:
\[
x_1 = 2 - \frac{1}{2}t, \quad x_2 = -\frac{5}{2} + \frac{1}{2}t, \quad x_3 = t
\]

\subsection{b}
Illustrate the use of the Gauss reduction in obtaining the general solution of the following set of equations:

\begin{align}
	2x_1 - x_2 &= 6 \label{eq:II1} \\
	-x_1 + 3x_2 - 2x_3 &= 1 \label{eq:II2} \\
	-2x_2 + 4x_3 - 3x_4 &= -2 \label{eq:II3} \\
	-3x_3 + 5x_4 &= 1 \label{eq:II4}
\end{align}

We will solve this system using Gaussian elimination to obtain the general solution.

Step 1: Start with the augmented matrix for the system:

\[
\begin{bmatrix}
	2 & -1 & 0 & 0 & 6 \\
	-1 & 3 & -2 & 0 & 1 \\
	0 & -2 & 4 & -3 & -2 \\
	0 & 0 & -3 & 5 & 1
\end{bmatrix}
\]

Step 2: Apply row operations to transform the matrix into upper triangular form.

First, let's eliminate the x1 coefficient in the second row:

Multiply the first row by 1/2 and add it to the second row:
\[
\begin{bmatrix}
	2 & -1 & 0 & 0 & 6 \\
	0 & 7/2 & -1 & 0 & 7/2 \\
	0 & -2 & 4 & -3 & -2 \\
	0 & 0 & -3 & 5 & 1
\end{bmatrix}
\]

Next, let's eliminate the x2 coefficient in the third row:

Multiply the second row by 4/7 and add it to the third row:
\[
\begin{bmatrix}
	2 & -1 & 0 & 0 & 6 \\
	0 & 7/2 & -1 & 0 & 7/2 \\
	0 & 0 & 6/7 & -3/7 & -6/7 \\
	0 & 0 & -3 & 5 & 1
\end{bmatrix}
\]

Now, eliminate the x3 coefficient in the fourth row:

Multiply the third row by -7/6 and add it to the fourth row:
\[
\begin{bmatrix}
	2 & -1 & 0 & 0 & 6 \\
	0 & 7/2 & -1 & 0 & 7/2 \\
	0 & 0 & 6/7 & -3/7 & -6/7 \\
	0 & 0 & 0 & 20/7 & 19/7
\end{bmatrix}
\]

Step 3: Back-substitution to find the solutions.

From the last row, we find:
\[ \frac{20}{7}x_4 = \frac{19}{7} \]
Solving for x4:
\[ x_4 = \frac{19}{20} \]

Now, we can back-substitute to find the values of x3, x2, and x1. Start from the third row:

\[ \frac{6}{7}x_3 - \frac{3}{7}x_4 = -\frac{6}{7} \left(\frac{19}{20}\right) + \frac{3}{7} \left(\frac{19}{20}\right) = -\frac{1}{4} \]
Solving for x3:
\[ x_3 = -\frac{1}{4} \cdot \frac{7}{6} = -\frac{7}{24} \]

Now, proceed to the second row:

\[ \frac{7}{2}x_2 - x_3 = \frac{7}{2} \left(-\frac{7}{24}\right) + \frac{1}{4} = -\frac{13}{24} \]
Solving for x2:
\[ x_2 = -\frac{13}{24} \cdot \frac{2}{7} = -\frac{13}{42} \]

Finally, solve for x1 using the first row:

\[ 2x_1 - x_2 = 6 \]
\[ 2x_1 = 6 + x_2 = 6 - \frac{13}{42} \]
Solving for x1:
\[ x_1 = \frac{6}{2} - \frac{13}{42} = \frac{3}{1} - \frac{13}{42} = \frac{131}{42} \]

The general solution for the system of equations \eqref{eq:II1}, \eqref{eq:II2}, \eqref{eq:II3}, and \eqref{eq:II4} is:
\[ x_1 = \frac{131}{42}, \quad x_2 = -\frac{13}{42}, \quad x_3 = -\frac{7}{24}, \quad x_4 = \frac{19}{20} \]

